rewrite fsum for the purpose of configurations

src/computability/fsum.lean
@@ -8,13 +8,21 @@ import tactic.basic
 import data.fintype.basic
 
 def quot.lift_on' {α : Type*} [s : setoid α]
-{t : α → Type*} {ht : ∀ a b : α, a ≈ b → t a = t b}
-(f : ∀ a : α, t a) (hf : ∀ a b : α, a ≈ b → f a == f b) : ∀ q : quotient s, quot.lift_on q t ht :=
-λ q, quotient.hrec_on q f hf
+{t : α → Type*} {C : Type* → Type*} {ht : ∀ a b : α, a ≈ b → t a = t b}
+(f : ∀ a : α, C (t a)) (hf : ∀ a b : α, a ≈ b → f a == f b) :
+∀ q : quotient s, C (quot.lift_on q t ht) := λ q, quotient.hrec_on q f hf
 
-def sum.elim' {α β: Type*} {tα : α → Type*} {tβ : β → Type*} (f : ∀ x, tα x) (g : ∀ x, tβ x) :
-∀ x : α ⊕ β, sum.elim tα tβ x := λ x, sum.cases_on x (λ y, f y) (λ y, g y)
+/-def sum.elim' {α β: Type*} {tα : α → Type*} {tβ : β → Type*} (f : ∀ x, tα x) (g : ∀ x, tβ x) :
+∀ x : α ⊕ β, sum.elim tα tβ x := λ x, sum.cases_on x f g-/
 
+def sum.elim' {α β: Type*} {tα : α → Type*} {tβ : β → Type*} {C : Type* → Type*}
+(f : ∀ x, C (tα x)) (g : ∀ x, C (tβ x)) :
+∀ x : α ⊕ β, C (sum.elim tα tβ x) := λ x, sum.cases_on x f g
+
+@[simp] lemma sum.elim_inl' {α β : Type*} {tα : α → Type*} {tβ : β → Type*} {C : Type* → Type*}
+(f : ∀ x, C (tα x)) (g : ∀ x, C (tβ x)) (x : α) : sum.elim' f g (sum.inl x) = f x := rfl
+@[simp] lemma sum.elim_inr' {α β : Type*} {tα : α → Type*} {tβ : β → Type*} {C : Type* → Type*}
+(f : ∀ x, C (tα x)) (g : ∀ x, C (tβ x)) (y : β) : sum.elim' f g (sum.inr y) = g y := rfl
 
 namespace fsum
 section
@@ -64,34 +72,154 @@ def elim_rel {γ : Type*} (f : α ⊕ β → γ) (h : f (sum.inl a) = f (sum.inr
 ∀ x y, fsum_rel x y → f x = f y := by tidy
 def elim_aux {γ : Type*} (f : α ⊕ β → γ) (h : f (sum.inl a) = f (sum.inr b)) : fsum → γ :=
 λ q, quot.lift_on q f (elim_rel f h)
-
 def elim {γ : Type*} (f : α → γ) (g : β → γ) (h : f a = g b) : fsum → γ :=
 elim_aux (sum.elim f g) h
+
+/--/
+def liftl' [hβ : decidable_eq β] (x : α ⊕ β) : α ⊕ β :=
+sum.cases_on x (λ x, sum.inl x) (λ y, ite (y = b) (sum.inl a) (sum.inr y))
+lemma liftl_nb' [hβ : decidable_eq β] (x : α ⊕ β) : liftl' x ≠ sum.inr b :=
+begin
+  cases x; unfold liftl',
+  apply sum.no_confusion,
+  intro h,
+  cases em (x = b) with e e, {
+    rw if_pos e at h,
+    exact sum.no_confusion h,
+  },
+  rw if_neg e at h,
+  apply e,
+  exact sum.inr.inj h,
+end
+
+def liftl [hβ : decidable_eq β] (q : fsum) : α ⊕ β :=
+elim_aux (λ x, liftl' x) begin
+  unfold liftl',
+  rw if_pos,
+  refl,
+end q
+
+lemma liftl_nb [hβ : decidable_eq β] (q : fsum) : liftl q ≠ sum.inr b :=
+begin
+  sorry,
+end-/
+
+def liftr [hα : decidable_eq α] (q : fsum) : α ⊕ β := begin
+  induction q,
+  cases q with x y h,
+  exact ite (x = a) (sum.inr b) (sum.inl x),
+  exact sum.inr y,
+  tidy,
+end
 
 @[simp] lemma elim_inl {γ : Type*} (f : α → γ) (g : β → γ)
 {h : f a = g b} (x : α) : elim f g h (inl x) = f x := rfl
 @[simp] lemma elim_inr {γ : Type*} (f : α → γ) (g : β → γ)
 {h : f a = g b} (y : β) : elim f g h (inr y) = g y := rfl
 
-def elim_rel' {t : α ⊕ β → Type*} {ht : t (sum.inl a) = t (sum.inr b)}
-(f : ∀ x : α ⊕ β, t x) (hf : f (sum.inl a) == f (sum.inr b)) : ∀ x y, fsum_rel x y → f x == f y := by tidy
-def elim_aux' {t : α ⊕ β → Type*} {ht : t (sum.inl a) = t (sum.inr b)}
-(f : ∀ x : α ⊕ β, t x) (hf : f (sum.inl a) == f (sum.inr b)) : ∀ x : fsum, elim_aux t ht x :=
-@quot.lift_on' _ fsum_setoid t (elim_rel t ht) f (@elim_rel' t ht f hf)
+def eliml [hβ : decidable_eq β] {γ : Type*} (f : α → γ) (g : β → γ) : fsum → γ :=
+elim_aux (sum.elim f (λ y, ite (y = b) (f a) (g y))) (by simp)
+def elimr [hα : decidable_eq α] {γ : Type*} (f : α → γ) (g : β → γ) : fsum → γ :=
+elim_aux (sum.elim (λ x, ite (x = a) (g b) (f x)) g) (by simp)
 
-def elim' {t₁ : α → Type*} {t₂ : β → Type*} {ht : t₁ a = t₂ b}
-(f : ∀ x : α, t₁ x) (g : ∀ x : β, t₂ x) (hf : f a == g b) : ∀ x : fsum, elim t₁ t₂ ht x :=
-@elim_aux' (sum.elim t₁ t₂) ht (sum.elim' f g) hf
+set_option pp.proofs true
+
+@[simp] lemma eliml_inl [hβ : decidable_eq β] {γ : Type*} (f : α → γ) (g : β → γ) (x : α):
+eliml f g (inl x) = f x := by refl
+@[simp] lemma elimr_inr [hα : decidable_eq α] {γ : Type*} (f : α → γ) (g : β → γ) (y : β):
+elimr f g (inr y) = g y := by refl
+
+lemma eliml_eq_elim [hβ : decidable_eq β] {γ : Type*} (f : α → γ) (g : β → γ) (h : f a = g b):
+eliml f g = elim f g h := begin
+  unfold eliml elim,
+  suffices h' : (λ (y : β), ite (y = b) (f a) (g y)) = g, {
+    simp [h'],
+    rw proof_irrel h,
+  },
+  ext y,
+  cases em (y = b) with h' h', {
+    rw [if_pos h',h'],
+    exact h,
+  },
+  rw if_neg h',
+end
+
+lemma elimr_eq_elim [hα : decidable_eq α] {γ : Type*} (f : α → γ) (g : β → γ) (h : f a = g b):
+elimr f g = elim f g h := begin
+  unfold elimr elim,
+  suffices h' : (λ (x : α), ite (x = a) (g b) (f x)) = f, {
+    simp [h'],
+    rw proof_irrel h,
+  },
+  ext x,
+  cases em (x = a) with h' h', {
+    rw [if_pos h',h'],
+    symmetry,
+    exact h,
+  },
+  rw if_neg h',
+end
+
+def elim_prod_rel {t : α ⊕ β → Type*} {C : Type* → Type*} {ht : t (sum.inl a) = t (sum.inr b)}
+(f : ∀ x : α ⊕ β, C (t x)) (hf : f (sum.inl a) == f (sum.inr b)) : ∀ x y, fsum_rel x y → f x == f y := by tidy
+def elim_prod_aux {t : α ⊕ β → Type*} {C : Type* → Type*} {ht : t (sum.inl a) = t (sum.inr b)}
+(f : ∀ x : α ⊕ β, C (t x)) (hf : f (sum.inl a) == f (sum.inr b)) : ∀ x : fsum, C (elim_aux t ht x) :=
+@quot.lift_on' _ fsum_setoid t C (elim_rel t ht) f (@elim_prod_rel t C ht f hf)
+def elim_prod {t₁ : α → Type*} {t₂ : β → Type*} {C : Type* → Type*} {ht : t₁ a = t₂ b}
+(f : ∀ x : α, C (t₁ x)) (g : ∀ x : β, C (t₂ x)) (hf : f a == g b) : ∀ x : fsum, C (elim t₁ t₂ ht x) :=
+@elim_prod_aux (sum.elim t₁ t₂) C ht (sum.elim' f g) hf
+
+
+def eliml_prod [hβ : decidable_eq β] {t₁ : α → Type*} {t₂ : β → Type*} {C : Type* → Type*}
+(f : ∀ x : α, C (t₁ x)) (g : ∀ y : β, C (t₂ y)) : ∀ q : fsum, C (eliml t₁ t₂ q) :=
+elim_prod_aux (sum.elim' f (λ y, dite (y = b)
+(λ h, by{ rw if_pos h, exact f a }) (λ h, by{ rw if_neg h, exact g y })))
+(by{ apply heq.symm, simp })
+
+def elimr_prod [hα : decidable_eq α] {t₁ : α → Type*} {t₂ : β → Type*} {C : Type* → Type*}
+(f : ∀ x : α, C (t₁ x)) (g : ∀ y : β, C (t₂ y)) : ∀ q : fsum, C (elimr t₁ t₂ q) :=
+elim_prod_aux (sum.elim' (λ x, dite (x = a)
+(λ h, by{ rw if_pos h, exact g b}) (λ h, by{ rw if_neg h, exact f x})) g)
+(by simp)
+
+
+def extendl_value {γ : Type*} [h : decidable_eq β] (f : α → γ) (c : γ) : fsum → γ :=
+elim f (λ y, ite (y = b) (f a) c) (by {rw if_pos, refl})
+def extendr_value {γ : Type*} [h : decidable_eq α] (g : β → γ) (c : γ) : fsum → γ :=
+elim (λ x, ite (x = a) (g b) c) g (by {rw if_pos, refl})
+
+def extendl {γ : Type*} (f : α → γ) : fsum → γ := elim f (λ y, f a) rfl
+def extendr {γ : Type*} (g : β → γ) : fsum → γ := elim (λ y, g b) g rfl
+
+def extendl_prod {γ : Type*} {t : α → Type*} {C : Type* → Type*} (f : ∀ x : α, C (t x))
+: ∀ q : fsum, C (extendl t q) := elim_prod f (λ y, f a) (congr_arg_heq f rfl)
+def extendr_prod {γ : Type*} {t : β → Type*} {C : Type* → Type*} (g : ∀ y : β, C (t y))
+: ∀ q : fsum, C (extendr t q) := elim_prod (λ x, g b) g (congr_arg_heq g rfl)
+
 
 instance inhabited_fsum : inhabited fsum := ⟨inl a⟩
 instance decidable_eq_fsum [dα : decidable_eq α] [dβ : decidable_eq β] : decidable_eq fsum :=
 @quotient.decidable_eq (α ⊕ β) fsum_setoid fsum_setoid.decidable_rel
-
-instance fintype [hα : fintype α] [hβ : fintype β] [hα' : decidable_eq α] [hβ' : decidable_eq β] :
+instance fintype_fsum [hα : fintype α] [hβ : fintype β] [hα' : decidable_eq α] [hβ' : decidable_eq β] :
 fintype fsum := @quotient.fintype _ (sum.fintype α β) fsum_setoid fsum_setoid.decidable_rel
 
 end
+
+def inl' {α β : Type*} {a : α} {b : β} (x : α) : fsum a b := inl a b x
+def inr' {α β : Type*} {a : α} {b : β} (y : β) : fsum a b := inr a b y
+def extendl' {α β γ : Type*} {a : α} {b : β} (f : α → γ) : fsum a b → γ := extendl a b f
+def extendr' {α β γ : Type*} {a : α} {b : β} (g : β → γ) : fsum a b → γ := extendr a b g
+
+lemma point_eq' {α β : Type*} {a : α} {b : β}: @inl' _ _ a b a = inr' b := point_eq a b
+
 end fsum
+
+def map_rec_codomain {α : Type*} {t₁ t₂ : α → Type*} (ft : ∀ a : α, t₁ a → t₂ a) (f : ∀ a : α, t₁ a)
+: ∀ a : α, t₂ a := λ a, ft a (f a)
+
+def map_rec_domain {α β : Type*} {t₁ : α → Type*} {t₂ : β → Type*} (ft : α → β)
+(h : ∀ a : α, t₁ a = t₂ (ft a)) (f : ∀ b : β, t₂ b) : ∀ a : α, t₁ a := λ a,
+begin rw h a, exact f (ft a), end
 
 
 /-
