src/computability/tm_composition.lean
@@ -6,80 +6,136 @@ Authors: Pim Spelier, Daan van Gent.
 
 import computability.encoding
 import computability.tm_computable
+import computability.fsum
+import data.list.basic
 
-namespace computability
+namespace turing
 
-private def fsum_setoid {α β : Type*} (a : α) (b : β) : setoid (α ⊕ β) := {
-  r := λ u v, sum.cases_on u
-    (λ x, sum.cases_on v
-      (λ y, x = y)
-      (λ y, (x = a) ∧ (y = b)))
-    (λ x, sum.cases_on v
-      (λ y, (x = b) ∧ (y = a))
-      (λ y, x = y)),
-  iseqv := by tidy }
+namespace composition
+noncomputable theory
 
-instance fsum_setoid.decidable_rel {α β : Type*} (a : α) (b : β) [dα : decidable_eq α] [dβ : decidable_eq β]:
-decidable_rel (fsum_setoid a b).r := begin
-  intros x y,
-  cases x; cases y,
-  exact dα x y,
-  exact and.decidable,
-  exact and.decidable,
-  exact dβ x y,
-end
+section computer
+open turing.TM2
+open turing.TM2.stmt
+open fsum
 
-def fsum {α β : Type*} (a : α) (b : β) : Type* := quotient (fsum_setoid a b)
+parameters (tm₂ tm₁ : fin_tm2) (hΓ : tm₂.Γ tm₂.k₀ = tm₁.Γ tm₁.k₁)
+instance dK₁ : _ := tm₁.K_decidable_eq
+instance dK₂ : _ := tm₂.K_decidable_eq
+instance dK : _ := fsum.decidable_eq_fsum tm₂.k₀ tm₁.k₁
+-- instance temp : fintype (fintype (fsum tm₂.k₀ tm₁.k₁)) := sorry
+-- instance temp' : fintype (fintype (tm₂.Λ ⊕ tm₁.Λ)) := sorry
 
-def fsum.inl {α β : Type*} {a : α} {b : β} (x : α) : fsum a b := quotient.mk' (sum.inl x)
-def fsum.inr {α β : Type*} {a : α} {b : β} (y : β) : fsum a b := quotient.mk' (sum.inr y)
+private def embed_tm₂_stmt : fin_tm2.stmt tm₂ →
+stmt (elim _ _ tm₂.Γ tm₁.Γ hΓ) (tm₂.Λ ⊕ tm₁.Λ) (fsum tm₂.initial_state tm₁.initial_state)
+| (push k f q) := push (inl' k) (extendl' f) (embed_tm₂_stmt q)
+| (peek k f q) := peek (inl' k) (extendl' (λ s g, inl' (f s g))) (embed_tm₂_stmt q)
+| (pop k f q) := pop (inl' k) (extendl' (λ s g, inl' (f s g))) (embed_tm₂_stmt q)
+| (load f q) := load (extendl' (inl' ∘ f)) (embed_tm₂_stmt q)
+| (branch f q r) := branch (extendl' f) (embed_tm₂_stmt q) (embed_tm₂_stmt r)
+| (goto f) := goto (extendl' (sum.inl ∘ f))
+| (halt) := halt
 
-def fsum.elim {α β γ : Type*} {a : α} {b : β} (f : α → γ) (g : β → γ) (h : f a = g b): fsum a b → γ := λ x,
-begin
-  apply quot.lift_on x (sum.elim f g) (λ u v h',
-  begin
-    cases u; cases v,
-    {
-      exact congr_arg (sum.elim f g) (congr_arg sum.inl h'),
-    }, {
-      suffices h'' : (u = a) ∧ (v = b),
-      simp only [h, h'', sum.elim_inl, sum.elim_inr],
-      exact h',
-    }, {
-      suffices h'' : (u = b) ∧ (v = a),
-      simp only [h, h'', sum.elim_inl, sum.elim_inr],
-      exact h',
-    }, {
-      exact congr_arg (sum.elim f g) (congr_arg sum.inr h'),
-    }
-  end),
-end
+private def embed_tm₁_stmt : fin_tm2.stmt tm₁ →
+stmt (elim _ _ tm₂.Γ tm₁.Γ hΓ) (tm₂.Λ ⊕ tm₁.Λ) (fsum tm₂.initial_state tm₁.initial_state)
+| (push k f q) := push (inr' k) (extendr' f) (embed_tm₁_stmt q)
+| (peek k f q) := peek (inr' k) (extendr' (λ s g, inr' (f s g))) (embed_tm₁_stmt q)
+| (pop k f q) := pop (inr' k) (extendr' (λ s g, inr' (f s g))) (embed_tm₁_stmt q)
+| (load f q) := load (extendr' (inr' ∘ f)) (embed_tm₁_stmt q)
+| (branch f q r) := branch (extendr' f) (embed_tm₁_stmt q) (embed_tm₁_stmt r)
+| (goto f) := goto (extendr' (sum.inr ∘ f))
+| (halt) := goto (λ s, sum.inl tm₂.main )
 
-instance fsum.inhabited {α β : Type*} (a : α) (b : β): inhabited (fsum a b) := ⟨fsum.inl a⟩
-instance fsum.decidable_eq {α β : Type*} [dα : decidable_eq α] [dβ : decidable_eq β] (a : α) (b : β): decidable_eq (fsum a b) :=
-@quotient.decidable_eq (α ⊕ β) (fsum_setoid a b) (fsum_setoid.decidable_rel a b)
-instance fsum.fintype {α β : Type*} (a : α) (b : β) [hα : fintype α] [hβ : fintype β]
-[hα' : decidable_eq α] [hβ' : decidable_eq β]: fintype (fsum a b) :=
-@quotient.fintype _ (sum.fintype α β) (fsum_setoid a b) (fsum_setoid.decidable_rel a b)
+-- class findeq (α : Type*) := ( fin : fintype α ) ( deq : decidable_eq α )
 
-noncomputable
-
-
-
-def fin_tm_comp (tm₂ tm₁ : fin_tm2) (hΓ : tm₂.Γ tm₂.k₀ = tm₁.Γ tm₁.k₁) : fin_tm2 := {
+def computer : fin_tm2 := {
   K := fsum tm₂.k₀ tm₁.k₁,
-  K_decidable_eq := @fsum.decidable_eq _ _ (tm₂.K_decidable_eq) (tm₁.K_decidable_eq) _ _,
-  k₀ := fsum.inr tm₁.k₀,
-  k₁ := fsum.inl tm₂.k₁,
-  Γ := fsum.elim tm₂.Γ tm₁.Γ hΓ,
+  K_decidable_eq := dK,
+  K_fin := @fsum.fintype_fsum _ _ _ _ tm₂.K_fin tm₁.K_fin tm₂.K_decidable_eq tm₁.K_decidable_eq,
+  k₀ := inr' tm₁.k₀,
+  k₁ := inl' tm₂.k₁,
+  Γ := elim _ _ tm₂.Γ tm₁.Γ hΓ,
   Λ := tm₂.Λ ⊕ tm₁.Λ,
   main := sum.inr tm₁.main,
+  Λ_fin := @sum.fintype tm₂.Λ tm₁.Λ tm₂.Λ_fin tm₁.Λ_fin,
   σ := fsum tm₂.initial_state tm₁.initial_state,
-  initial_state := fsum.inr tm₁.initial_state,
-  σ_fin := @fsum.fintype _ _ _ _ tm₂.σ_fin tm₁.σ_fin (classical.dec_eq tm₂.σ) (classical.dec_eq tm₁.σ), -- Horror!
+  initial_state := inr' tm₁.initial_state,
+  σ_fin := @fsum.fintype_fsum _ _ _ _ tm₂.σ_fin tm₁.σ_fin (classical.dec_eq tm₂.σ) (classical.dec_eq tm₁.σ), -- Horror!
   Γk₀_fin := tm₁.Γk₀_fin,
-  M := λ (l : tm₂.Λ ⊕ tm₁.Λ), sorry
+  M := sum.elim (embed_tm₂_stmt ∘ tm₂.M) (embed_tm₁_stmt ∘ tm₁.M)
 }
 
+def embed_tm₁_cfg (c : fin_tm2.cfg tm₁): fin_tm2.cfg computer := {
+  l := (option.map sum.inr) c.l,
+  var := inr' c.var,
+  stk := begin
+    let h := elimr_prod tm₂.k₀ tm₁.k₁ (λ k, @list.nil (tm₂.Γ k)) c.stk,
+    rw elimr_eq_elim tm₂.k₀ tm₁.k₁ tm₂.Γ tm₁.Γ hΓ at h,
+    exact h,
+  end
+}
 
-end computability
+def embed_tm₂_cfg (c : fin_tm2.cfg tm₂): fin_tm2.cfg computer := {
+  l := (option.map sum.inl) c.l,
+  var := inl' c.var,
+  stk := begin
+    let h := eliml_prod tm₂.k₀ tm₁.k₁ c.stk (λ k, @list.nil (tm₁.Γ k)),
+    rw eliml_eq_elim tm₂.k₀ tm₁.k₁ tm₂.Γ tm₁.Γ hΓ at h,
+    exact h,
+  end
+}
+
+end computer
+
+open computability
+
+lemma center_stack {α β γ : Type} (eα : fin_encoding α) (eβ : fin_encoding β) (eγ : fin_encoding γ)
+(g : β → γ) (f : α → β) (hg : tm2_computable eβ eγ g) (hf : tm2_computable eα eβ f) :
+hg.to_tm2_computable_aux.tm.Γ hg.to_tm2_computable_aux.tm.k₀ = hf.to_tm2_computable_aux.tm.Γ hf.to_tm2_computable_aux.tm.k₁ :=
+begin
+
+end
+
+theorem X {α β γ : Type} (eα : fin_encoding α) (eβ : fin_encoding β) (eγ : fin_encoding γ)
+(g : β → γ) (f : α → β) (hg : tm2_computable eβ eγ g) (hf : tm2_computable eα eβ f) :
+tm2_computable eα eγ (g ∘ f) := {
+  tm := computer hg.tm hf.tm begin end, -- !!!
+  input_alphabet := hf.input_alphabet,
+  output_alphabet := hg.output_alphabet,
+  outputs_fun := λ a, {
+    steps := (hg.outputs_fun (f a)).steps + (hf.outputs_fun a).steps,
+    evals_in_steps := begin
+      --suffices h : ((flip bind f)^[(hg.outputs_fun (f a)).steps] a) = some (f a)
+
+      let tm₁ := hf.tm,
+      let tm₂ := hg.tm,
+      have hΓ : tm₂.Γ tm₂.k₀ = tm₁.Γ tm₁.k₁ := sorry,
+      let tm := computer tm₂ tm₁ hΓ,
+      let alph1 := hf.input_alphabet,
+      let alph2 := hf.output_alphabet,
+      let alph3 := hg.output_alphabet,
+
+      /-have hΓ' : hf.to_computable_by_tm2_aux.tm.Γ hf.to_computable_by_tm2_aux.tm.k₁ = tm.Γ tm.k₁ :=
+      begin
+        change tm₁.Γ tm₁.k₁ = tm.Γ tm.k₁,
+        -- have fsum.elim tm₂.Γ tm₁.Γ hΓ (fsum.inl tm₂.k₁) = tm.Γ tm.k₁,
+
+        --change fsum.elim hg.tm.Γ hf.tm.Γ sorry
+        --exact fsum.elim_inl hf.tm.Γ _ _ tm.k₁,
+      end-/
+      let la := (list.map alph1.inv_fun (eα.encode a)),
+      let lb := (list.map alph2.inv_fun (eβ.encode (f a))),
+      let lc := (list.map alph3.inv_fun (eγ.encode ((g ∘ f) a))),
+
+      have h : evals_to tm.step (init_list tm la) ((option.map (halt_list tm)) (some lb)),
+      sorry,
+      --evals_to tm.step (init_list tm l) ((option.map (halt_list tm)) l')
+    end
+}}
+
+
+--lemma X (l : list (computer.Γ computer.k₀)) (l' : option (list (computer.Γ computer.k₁))) (o₂ : tm2_outputs tm₂ l l' )
+--(l : list (tm.Γ tm.k₀)) (l' : option (list (tm.Γ tm.k₁))) :=
+
+end composition
+end turing
